Progress with closure semantics + equivalence proof

src/Env/Semantics.v
@@ -2,21 +2,20 @@ From CoreErlang Require Export Env.Syntax.
 Import ListNotations.
 Open Scope env_scope.
 
+Definition Env := list Val.
 
 Inductive Frame : Set :=
-| FApp1 (l : list Exp) (* apply □(e₁, e₂, ..., eₙ) *)
-| FBIF1 (l : list Exp) (* call □(e₁, e₂, ..., eₙ) *)
-| FLet (e2 : Exp) (* let v = □ in e2 *)
-| FCase (p : Pat) (e2 e3 : Exp) (* if □ then e2 else e3 *)
-| FCons1 (e1 : Exp) (* [e1 | □] *)
-| FCons2 (v2 : Val) (* [□ | v2] *)
+| FApp1 (l : list Exp) (Γ : Env) (* apply □(e₁, e₂, ..., eₙ) *)
+| FBIF1 (l : list Exp) (Γ : Env) (* call □(e₁, e₂, ..., eₙ) *)
+| FLet (e2 : Exp) (Γ : Env) (* let v = □ in e2 *)
+| FCase (p : Pat) (e2 e3 : Exp) (Γ : Env) (* if □ then e2 else e3 *)
+| FCons1 (e1 : Exp) (Γ : Env) (* [e1 | □] *)
+| FCons2 (v2 : Val) (Γ : Env) (* [□ | v2] *)
 
-| FApp2 (v : Val) (l : list Val) (el : list Exp)
-| FBIF2 (v : Val) (l : list Val) (el : list Exp).
+| FApp2 (v : Val) (l : list Val) (el : list Exp) (Γ : Env)
+| FBIF2 (v : Val) (l : list Val) (el : list Exp) (Γ : Env).
 
 Definition FrameStack := list Frame.
-
-Definition Environment := list Val.
 
 Definition eval (f : Val) (l : list Val) : option Val :=
 match f with
@@ -28,7 +27,7 @@ match f with
 | _ => None
 end.
 
-Definition beta_reduce (f : Val) (params : list Val) : option (Environment * Exp) :=
+Definition beta_reduce (f : Val) (params : list Val) : option (Env * Exp) :=
 match f with
 | VClos Γ arity body =>
     if Nat.eqb (length params) arity then
@@ -38,63 +37,130 @@ match f with
 end.
 
 
-Reserved Notation "⟨ G , fs , e ⟩ --> ⟨ G' , fs' , e' ⟩" (at level 50).
-Inductive step : Environment -> FrameStack -> Exp -> Environment -> FrameStack -> Exp -> Prop :=
-(**  Reduction rules *)
-| red_bif0 Γ xs v res:
+(*
+
+Inductive heat : Env -> Exp -> Frame -> Exp -> Prop :=
+
+
+Reserved Notation "⟨ F , v ⟩ -->ᶜ ⟨ G , e ⟩" (at level 50).
+Inductive cool : Frame -> Val -> Env -> Exp -> Prop :=
+
+| cool_bif0 Γ xs v res:
   eval v [] = Some res ->
   ⟨ Γ , (FBIF1 [])::xs, ˝v ⟩ --> ⟨ Γ, xs , res⟩
 
-| red_bif Γ xs e1 l v:
+| cool_bif Γ xs e1 l v:
   ⟨ Γ , (FBIF1 (e1::l))::xs, ˝v ⟩ --> ⟨ Γ, FBIF2 v [] l :: xs, e1 ⟩
 
-| step_bif_params Γ xs vl e1 el v v0:
+| cool_bif_params Γ xs vl e1 el v v0:
   ⟨ Γ , (FBIF2 v vl (e1::el))::xs, ˝v0 ⟩ --> ⟨ Γ, FBIF2 v (v0 :: vl) el :: xs, e1 ⟩
 
-| red_bif_params Γ xs vl v v0 res:
+| cool_bif_params Γ xs vl v v0 res:
   eval v (vl ++ [v0]) = Some res ->
   ⟨ Γ , (FBIF2 v vl [])::xs, ˝v0 ⟩ --> ⟨ Γ, xs, res ⟩
 
-| red_app0 Γ xs v Γ' res:
+| cool_app0 Γ xs v Γ' res:
   beta_reduce v [] = Some (Γ', res) ->
   ⟨ Γ , (FApp1 [])::xs, ˝v ⟩ --> ⟨ Γ', xs , res⟩
 
-| red_app Γ xs e1 l v:
+| cool_app Γ xs e1 l v:
   ⟨ Γ , (FApp1 (e1::l))::xs, ˝v ⟩ --> ⟨ Γ, FApp2 v [] l :: xs, e1 ⟩
 
 | step_app_params Γ xs vl e1 el v v0:
   ⟨ Γ , (FApp2 v vl (e1::el))::xs, ˝v0 ⟩ --> ⟨ Γ, FApp2 v (v0 :: vl) el :: xs, e1 ⟩
 
-| red_app_params Γ xs vl v v0 Γ' res:
+| cool_app_params Γ xs vl v v0 Γ' res:
   beta_reduce v (vl ++ [v0]) = Some (Γ', res) ->
   ⟨ Γ , (FApp2 v vl [])::xs, ˝v0 ⟩ --> ⟨ Γ', xs, res ⟩
 
 
-| red_let Γ val e2 xs :
+| cool_let Γ val e2 xs :
   ⟨ Γ , (FLet e2)::xs, ˝val ⟩ --> ⟨ val :: Γ, xs, e2 ⟩
 
-| red_case_true Γ e2 e3 v p xs l : 
+| cool_case_true Γ e2 e3 v p xs l : 
   match_pattern p v = Some l
 ->
   ⟨ Γ, (FCase p e2 e3)::xs, ˝v ⟩ --> ⟨ l ++ Γ, xs, e2 ⟩
 
-| red_case_false Γ e2 e3 p v xs :
+| cool_case_false Γ e2 e3 p v xs :
   match_pattern p v = None ->
   ⟨ Γ, (FCase p e2 e3)::xs, ˝v ⟩ --> ⟨ Γ, xs, e3 ⟩
 
-| red_cons1 Γ xs v2 e1 :
+| cool_cons1 Γ xs v2 e1 :
   ⟨ Γ, FCons1 e1::xs, ˝v2⟩ --> ⟨Γ,FCons2 v2::xs, e1 ⟩
 
-| red_cons2 Γ xs v2 v1 :
+| cool_cons2 Γ xs v2 v1 :
   ⟨ Γ,FCons2 v2::xs, ˝v1⟩ --> ⟨Γ,xs, VCons v1 v2 ⟩
 
+where "⟨ F , v ⟩ -->ᶜ ⟨ G , e ⟩" := (cool F v G e).
+
+Reserved Notation "⟨ G , e ⟩ -->ˢ v" (at level 50).
+Inductive single : Env -> Exp -> Val -> Prop :=
+| red_fun Γ xs vl e:
+  ⟨Γ, EFun vl e⟩ -->ₛ VClos Γ vl e
+
+| red_var Γ xs x (val : Val) :
+  Γ !! x = Some val ->
+  ⟨Γ, VVar x⟩ -->ₛ val.
+where "⟨ G , e ⟩ -->ₛ v" := single G e v. *)
+
+Reserved Notation "⟨ G , fs , e ⟩ --> ⟨ G' , fs' , e' ⟩" (at level 50).
+Inductive step : Env -> FrameStack -> Exp -> Env -> FrameStack -> Exp -> Prop :=
+(**  Reduction rules *)
+| red_bif0 Γ0 Γ xs v res:
+  eval v [] = Some res ->
+  ⟨ Γ0 , (FBIF1 [] Γ)::xs, ˝v ⟩ --> ⟨ Γ, xs , res⟩
+
+| red_bif Γ0 Γ xs e1 l v:
+  ⟨ Γ0 , (FBIF1 (e1::l) Γ)::xs, ˝v ⟩ --> ⟨ Γ, FBIF2 v [] l Γ :: xs, e1 ⟩
+
+| step_bif_params Γ0 Γ xs vl e1 el v v0:
+  ⟨ Γ0 , (FBIF2 v vl (e1::el) Γ)::xs, ˝v0 ⟩ --> ⟨ Γ, FBIF2 v (vl ++ [v0]) el Γ :: xs, e1 ⟩
+
+| red_bif_params Γ0 Γ xs vl v v0 res:
+  eval v (vl ++ [v0]) = Some res ->
+  ⟨ Γ0 , (FBIF2 v vl [] Γ)::xs, ˝v0 ⟩ --> ⟨ Γ, xs, res ⟩
+
+| red_app0 Γ0 Γ xs v Γ' res:
+  beta_reduce v [] = Some (Γ', res) ->
+  ⟨ Γ0 , (FApp1 [] Γ)::xs, ˝v ⟩ --> ⟨ Γ', xs , res⟩
+
+| red_app Γ0 Γ xs e1 l v:
+  ⟨ Γ0 , (FApp1 (e1::l) Γ)::xs, ˝v ⟩ --> ⟨ Γ, FApp2 v [] l Γ :: xs, e1 ⟩
+
+| step_app_params Γ0 Γ xs vl e1 el v v0:
+  ⟨ Γ0 , (FApp2 v vl (e1::el) Γ)::xs, ˝v0 ⟩ --> ⟨ Γ, FApp2 v (vl ++ [v0]) el Γ :: xs, e1 ⟩
+
+| red_app_params Γ0 Γ xs vl v v0 Γ' res:
+  beta_reduce v (vl ++ [v0]) = Some (Γ', res) ->
+  ⟨ Γ0 , (FApp2 v vl [] Γ)::xs, ˝v0 ⟩ --> ⟨ Γ', xs, res ⟩
+
+
+| red_let Γ0 Γ val e2 xs :
+  ⟨ Γ0 , (FLet e2 Γ)::xs, ˝val ⟩ --> ⟨ val :: Γ, xs, e2 ⟩
+
+| red_case_true Γ0 Γ e2 e3 v p xs l : 
+  match_pattern p v = Some l
+->
+  ⟨ Γ0, (FCase p e2 e3 Γ)::xs, ˝v ⟩ --> ⟨ l ++ Γ, xs, e2 ⟩
+
+| red_case_false Γ0 Γ e2 e3 p v xs :
+  match_pattern p v = None ->
+  ⟨ Γ0, (FCase p e2 e3 Γ)::xs, ˝v ⟩ --> ⟨ Γ, xs, e3 ⟩
+
+| red_cons1 Γ0 Γ xs v2 e1 :
+  ⟨ Γ0, FCons1 e1 Γ::xs, ˝v2⟩ --> ⟨Γ,FCons2 v2 Γ::xs, e1 ⟩
+
+| red_cons2 Γ0 Γ xs v2 v1 :
+  ⟨ Γ0,FCons2 v2 Γ::xs, ˝v1⟩ --> ⟨Γ,xs, VCons v1 v2 ⟩
+
 (** Steps *)
-| step_let Γ xs e1 e2 : ⟨ Γ,xs, ELet e1 e2 ⟩ --> ⟨ Γ,(FLet e2)::xs, e1 ⟩
-| step_app Γ xs e el: ⟨ Γ,xs, EApp e el ⟩ --> ⟨ Γ,(FApp1 el)::xs, e ⟩
+| step_let Γ xs e1 e2 : ⟨ Γ,xs, ELet e1 e2 ⟩ --> ⟨ Γ, (FLet e2 Γ)::xs, e1 ⟩
+| step_app Γ xs e el: ⟨ Γ,xs, EApp e el ⟩ --> ⟨ Γ,(FApp1 el Γ)::xs, e ⟩
 | step_bif Γ fs name params:
-  ⟨Γ,fs, EBIF name params⟩ --> ⟨Γ,FBIF1 params :: fs, name⟩
-| step_case Γ xs e1 p e2 e3 : ⟨ Γ,xs, ECase e1 p e2 e3⟩ --> ⟨ Γ,(FCase p e2 e3)::xs, e1⟩
-| step_cons Γ xs e1 e2: ⟨ Γ,xs, ECons e1 e2 ⟩ --> ⟨ Γ,(FCons1 e1) :: xs, e2 ⟩
+  ⟨Γ,fs, EBIF name params⟩ --> ⟨Γ,FBIF1 params Γ :: fs, name⟩
+| step_case Γ xs e1 p e2 e3 : ⟨ Γ,xs, ECase e1 p e2 e3⟩ --> ⟨ Γ,(FCase p e2 e3 Γ)::xs, e1⟩
+| step_cons Γ xs e1 e2: ⟨ Γ,xs, ECons e1 e2 ⟩ --> ⟨ Γ,(FCons1 e1 Γ) :: xs, e2 ⟩
 
 (** Additional rules to handle environments *)
 | red_fun Γ xs vl e:
@@ -103,14 +169,14 @@ Inductive step : Environment -> FrameStack -> Exp -> Environment -> FrameStack -
 | red_var Γ xs x (val : Val) :
   Γ !! x = Some val ->
   ⟨Γ, xs, VVar x⟩ --> ⟨Γ, xs, ˝val⟩
-where "⟨ G , fs , e ⟩ --> ⟨ G' , fs' , e' ⟩" := (step G fs e G' fs' e').
+where "⟨ G , fs , e ⟩ --> ⟨ G' , fs' , e' ⟩" := (step G fs e G' fs' e') : env_scope.
 
 Reserved Notation "⟨ G , fs , e ⟩ -[ k ]-> ⟨ G' , fs' , e' ⟩" (at level 50).
-Inductive step_rt : Environment -> FrameStack -> Exp -> nat -> Environment -> FrameStack -> Exp -> Prop :=
+Inductive step_rt : Env -> FrameStack -> Exp -> nat -> Env -> FrameStack -> Exp -> Prop :=
 | step_refl Γ e Fs : ⟨ Γ, Fs, e ⟩ -[ 0 ]-> ⟨ Γ, Fs, e ⟩
 | step_trans Γ fs e Γ' fs' e' Γ'' fs'' e'' k:
   ⟨ Γ, fs, e ⟩ --> ⟨ Γ', fs', e'⟩ -> ⟨Γ', fs', e'⟩ -[ k ]-> ⟨Γ'', fs'', e''⟩
 ->
   ⟨ Γ, fs, e ⟩ -[S k]-> ⟨Γ'', fs'', e''⟩
-where "⟨ G , fs , e ⟩ -[ k ]-> ⟨ G' , fs' , e' ⟩" := (step_rt G fs e k G' fs' e').
+where "⟨ G , fs , e ⟩ -[ k ]-> ⟨ G' , fs' , e' ⟩" := (step_rt G fs e k G' fs' e') : env_scope.
 
