src/SemanticProperties.v
@@ -1,0 +1,1554 @@
+
+(** Example, simple evaluations *)
+Open Scope Z_scope.
+Goal ⟨ [], inc 1 ⟩ -->* ELit 2.
+Proof.
+  repeat (econstructor;cbn).
+Qed.
+
+Local Goal ⟨ [], simplefun 10 ⟩ -->* ELit 10.
+Proof.
+  repeat econstructor.
+Qed.
+
+Local Goal ⟨ [], simplefun2 10 10 ⟩ -->* ELit 20.
+Proof.
+  unfold simplefun2.
+  repeat econstructor.
+  all: inversion H; subst; cbn in *; auto.
+  all: inversion H1; subst; cbn in *; auto; lia.
+Qed.
+
+Local Goal ⟨ [], sum 1 ⟩ -->* ELit 1%Z.
+Proof.
+  assert (VALCLOSED (EFun [XVar]
+             (ECase (EVar 1) (PLit 0) (EVar 1)
+                (EBIF (ELit "+"%string) [EVar 1; EApp (EFunId 0) [EBIF (ELit "+"%string) [EVar 1; ELit (-1)]]])))). {
+    do 3 constructor; auto.
+    intros. inversion H; subst; cbn. 2: inversion H1.
+    all: auto.
+    constructor; auto.
+    intros. inversion H0. 2: inversion H2.
+    constructor; auto.
+    intros. inversion H1. 2: inversion H4. 3: inversion H6.
+    all: cbn; auto.
+    lia.
+  }
+  unfold sum.
+  simpl.
+  constructor. constructor. econstructor.
+  econstructor.
+  econstructor.
+  econstructor. constructor. cbn. econstructor. constructor. auto.
+  econstructor.
+  eapply red_app2. constructor.
+  simpl. econstructor. econstructor. econstructor. cbn. eapply step_case.
+  econstructor. eapply red_case_false. constructor. constructor. cbn. congruence.
+  econstructor. eapply step_bif.
+  econstructor. eapply red_bif_start; auto.
+  econstructor. eapply red_bif_step; auto.
+  econstructor. cbn. eapply step_app.
+  econstructor. eapply red_app_start. auto.
+  econstructor.
+  eapply step_bif.
+
+  econstructor. eapply red_bif_start; auto.
+  econstructor. eapply red_bif_step; auto. simpl.
+  econstructor. eapply red_plus; auto. simpl.
+  econstructor. eapply red_app2. constructor.
+  simpl. econstructor. econstructor. econstructor. cbn. eapply step_case.
+  econstructor. eapply red_case_true. constructor. reflexivity.
+  econstructor. eapply red_plus.
+  econstructor.
+Qed.
+
+Local Goal ⟨[], ECons (EBIF (ELit "+"%string) [ELit 1; ELit 1]) (ECons (ELit 1) (ECons (ELit 0) ENil))⟩ -->* VCons (ELit 2) (VCons (ELit 1) (VCons (ELit 0) ENil)).
+Proof.
+  split. repeat constructor. exists 13%nat.
+  econstructor. constructor.
+  econstructor. apply step_cons.
+  econstructor. apply step_cons. econstructor. constructor. constructor.
+  econstructor. constructor; constructor.
+  econstructor. constructor. repeat constructor.
+  econstructor. constructor; repeat constructor.
+  econstructor. constructor. repeat constructor.
+  econstructor. apply step_bif.
+  econstructor. constructor. constructor.
+  econstructor. constructor.
+  econstructor. constructor. 1-2: repeat constructor.
+  repeat econstructor.
+Qed.
+
+(** Complex example for map *)
+Local Goal
+   ⟨[], obj_map (EFun [YVar] (EBIF (ELit "+"%string) [EVar 1; ELit 1]))
+                (ECons (ELit 0) (ECons (ELit 1) (ECons (ELit 2) ENil)))⟩ -->*
+   VCons (ELit 1) (VCons (ELit 2) (VCons (ELit 3) ENil)).
+Proof.
+  (** closedness assertions for the occuring functions *)
+  assert (VALCLOSED (EFun [FVar; XVar]
+             (ECase (EVar 2) (PCons PVar PVar)
+                (ECons (EApp (EVar 3) [EVar 0])
+                   (EApp (EFunId 2) [EVar 3; EVar 1])) ENil))). {
+    constructor. cbn. repeat constructor.
+                               all: destruct i.
+                               all: try destruct i. all: simpl in H; try lia.
+                               all: simpl; auto; constructor; lia.
+  }
+  assert (VALCLOSED (EFun [YVar] (EBIF (ELit "+"%string) [EVar 1; ELit 1]))). {
+    constructor. cbn. repeat constructor.
+                               all: destruct i.
+                               all: try destruct i.
+                               all: simpl; auto.
+                               simpl in H0. lia.
+  }
+  split; auto. exists 64%nat.
+
+  (** evaluate letrec *)
+  econstructor. constructor. simpl.
+
+  (** start application evaluation *)
+  econstructor. constructor. simpl.
+  econstructor. constructor. auto.
+
+  (** function parameter *)
+  econstructor. constructor; auto; simpl.
+
+  (** evaluate list to value list *)
+  simpl.
+  econstructor. apply step_cons; auto.
+  econstructor. apply step_cons; auto.
+  econstructor. apply step_cons; auto.
+  econstructor. apply red_cons1; auto.
+  econstructor. apply red_cons2; auto.
+  econstructor. apply red_cons1; auto.
+  econstructor. apply red_cons2; auto.
+  econstructor. apply red_cons1; auto.
+  econstructor. apply red_cons2; auto.
+
+  (** process first element in the recursive call *)
+  econstructor. constructor; auto. cbn.
+  econstructor. apply step_case; auto.
+  econstructor. constructor; auto. reflexivity. cbn.
+  econstructor. apply step_cons. auto. cbn.
+  econstructor. apply step_app.
+  econstructor. constructor. auto.
+  econstructor. constructor; auto. simpl.
+
+  (** process second element in the recursive call *)
+  econstructor. constructor; auto. cbn.
+  econstructor. apply step_case; auto.
+  econstructor. constructor; auto. reflexivity. cbn.
+  econstructor. apply step_cons. auto. cbn.
+  econstructor. apply step_app.
+  econstructor. constructor. auto.
+  econstructor. constructor; auto. simpl.
+
+  (** process third element in the recursive call *)
+  econstructor. constructor; auto. cbn.
+  econstructor. apply step_case; auto.
+  econstructor. constructor; auto. reflexivity. cbn.
+  econstructor. apply step_cons. auto. cbn.
+  econstructor. apply step_app.
+  econstructor. constructor. auto.
+  econstructor. constructor; auto. simpl.
+
+  (** stop recursion with ENil *)
+  econstructor. constructor; auto. cbn.
+  econstructor. apply step_case; auto.
+  econstructor. apply red_case_false; auto.
+
+  (** apply function to the third element *)
+  econstructor. constructor; auto.
+  econstructor. apply step_app; auto.
+  econstructor. constructor; auto.
+  econstructor. constructor; auto. cbn.
+  econstructor. apply step_bif; auto.
+  econstructor. constructor; auto.
+  econstructor. constructor; auto. cbn.
+  econstructor. constructor; auto. cbn.
+  econstructor. constructor; auto.
+
+  (** apply function to the second element *)
+  econstructor. constructor; auto.
+  econstructor. apply step_app; auto.
+  econstructor. constructor; auto.
+  econstructor. constructor; auto. cbn.
+  econstructor. apply step_bif; auto.
+  econstructor. constructor; auto.
+  econstructor. constructor; auto. cbn.
+  econstructor. constructor; auto. cbn.
+  econstructor. constructor; auto.
+
+  (** apply function to the first element *)
+  econstructor. constructor; auto.
+  econstructor. apply step_app; auto.
+  econstructor. constructor; auto.
+  econstructor. constructor; auto. cbn.
+  econstructor. apply step_bif; auto.
+  econstructor. constructor; auto.
+  econstructor. constructor; auto. cbn.
+  econstructor. constructor; auto. cbn.
+  econstructor. constructor; auto.
+  constructor.
+Qed.
+
+(** Complex example for foldr *)
+Local Goal
+   ⟨[], obj_foldr
+                (EFun [XVar;YVar] (ECons (EBIF (ELit "+"%string) [EVar 1; ELit 1]) (EVar 2)))
+                (ECons (ELit 0) (ECons (ELit 1) (ECons (ELit 2) ENil))) ENil⟩ -->*
+   VCons (ELit 1) (VCons (ELit 2) (VCons (ELit 3) ENil)).
+Proof.
+  (** closedness assertions for the occuring functions *)
+  assert (VALCLOSED (EFun [FVar; DVar; XVar]
+             (ECase (EVar 3) (PCons PVar PVar)
+                (EApp (EVar 3)
+                   [EVar 0; EApp (EFunId 2) [EVar 3; EVar 4; EVar 1]])
+                (EVar 2)))). {
+    constructor. cbn. do 2 constructor; auto.
+    repeat constructor; intros.
+    all: destruct i.
+    all: try destruct i. all: simpl in *; try lia.
+    all: intros.
+    1-2: simpl; auto; repeat constructor.
+    simpl in *.
+    destruct i. 2: destruct i. 3: destruct i. all: auto.
+    constructor. all: lia.
+  }
+  assert (VALCLOSED (EFun [XVar; YVar]
+             (ECons (EBIF (ELit "+"%string) [EVar 1; ELit 1]) (EVar 2)))). {
+    constructor. cbn. repeat constructor.
+    all: destruct i; simpl in *.
+    all: try destruct i. all: simpl in H; try lia.
+    all: simpl; auto; constructor; lia.
+  }
+  split; auto. exists 71%nat.
+
+  (** Evaluate letrec *)
+  econstructor. constructor. simpl.
+
+  (** Application with 3 params *)
+  econstructor. constructor. simpl.
+  econstructor. constructor. auto.
+  econstructor. constructor; auto. simpl.
+  econstructor. constructor; auto.
+
+  (** evaluate parameter list to list of values *)
+  econstructor. apply step_cons; auto.
+  econstructor. apply step_cons; auto.
+  econstructor. apply step_cons; auto.
+  econstructor. apply red_cons1; auto.
+  econstructor. apply red_cons2; auto.
+  econstructor. apply red_cons1; auto.
+  econstructor. apply red_cons2; auto.
+  econstructor. apply red_cons1; auto.
+  econstructor. apply red_cons2; auto. simpl.
+
+  (** apply recursive call with the first element *)
+  econstructor. constructor; auto. cbn.
+  econstructor. apply step_case; auto.
+  econstructor. constructor; auto. reflexivity. cbn.
+  econstructor. apply step_app.
+  econstructor. constructor. auto.
+  econstructor. constructor; auto. cbn.
+
+  (** apply recursive call with the second element *)
+  econstructor. apply step_app.
+  econstructor. constructor. auto.
+  econstructor. constructor; auto. cbn.
+  econstructor. constructor; auto. cbn.
+  econstructor. constructor; auto. cbn.
+  econstructor. apply step_case; auto.
+  econstructor. constructor; auto. reflexivity. cbn.
+  econstructor. apply step_app.
+  econstructor. constructor. auto.
+  econstructor. constructor; auto. cbn.
+
+  (** apply recursive call with the third element *)
+  econstructor. apply step_app.
+  econstructor. constructor. auto.
+  econstructor. constructor; auto. cbn.
+  econstructor. constructor; auto. cbn.
+  econstructor. constructor; auto. cbn.
+  econstructor. apply step_case; auto.
+  econstructor. constructor; auto. reflexivity. cbn.
+  econstructor. apply step_app.
+  econstructor. constructor. auto.
+  econstructor. constructor; auto. cbn.
+
+  (** end of recursion with ENil *)
+  econstructor. apply step_app.
+  econstructor. constructor; auto. cbn.
+  econstructor. constructor; auto. cbn.
+  econstructor. constructor; auto. cbn.
+  econstructor. constructor; auto. cbn.
+  econstructor. apply step_case; auto.
+  econstructor. apply red_case_false; auto.
+
+  (** build the list back, by applying the +1 BIF *)
+  (** 3rd element *)
+  econstructor. constructor; auto. cbn.
+  econstructor. apply step_cons.
+  econstructor. constructor; auto.
+  econstructor. apply step_bif.
+  econstructor. constructor; auto.
+  econstructor. constructor; auto. cbn.
+  econstructor. constructor; auto. cbn.
+  econstructor. constructor; auto. cbn.
+  econstructor. constructor; auto. cbn.
+  (** 2nd element *)
+  econstructor. apply step_cons.
+  econstructor. constructor. auto.
+  econstructor. apply step_bif.
+  econstructor. constructor; auto.
+  econstructor. constructor; auto. cbn.
+  econstructor. constructor; auto. cbn.
+  econstructor. constructor; auto. cbn.
+  econstructor. constructor; auto. cbn.
+  (** 1st element *)
+  econstructor. apply step_cons.
+  econstructor. constructor; auto.
+  econstructor. apply step_bif.
+  econstructor. constructor; auto.
+  econstructor. constructor; auto. cbn.
+  econstructor. constructor; auto. cbn.
+  econstructor. constructor; auto. cbn.
+  constructor.
+Qed.
+
+Definition computes (x : string) (e : Exp) (f : Exp -> Exp) :=
+  forall v, ⟨[], EApp (EFun [x] e) [v]⟩ -->* f v.
+
+Fixpoint cons_to_list (e : Exp) : option (list Exp) :=
+match e with
+| ENil => Some []
+| VCons e1 e2 => match cons_to_list e2 with
+                 | Some e2'=> Some (e1 :: e2')
+                 | _ => None
+                 end
+| _ => None
+end.
+
+Fixpoint list_to_cons (l : list Exp) : Exp :=
+match l with
+| [] => ENil
+| e1 :: xs => VCons e1 (list_to_cons xs)
+end.
+
+Ltac proof_irr :=
+match goal with
+| [H1 : ?P, H2 : ?P |- _] => assert (H1 = H2) by apply proof_irrelevance; subst
+end.
+Ltac proof_irr_many := repeat proof_irr.
+
+(** Properties of the semantics *)
+Theorem step_determinism {e e' fs fs'} :
+  ⟨ fs, e ⟩ --> ⟨fs', e'⟩ ->
+  (forall fs'' e'', ⟨fs, e⟩ --> ⟨fs'', e''⟩ -> fs'' = fs' /\ e'' = e').
+Proof.
+  intro H. dependent induction H; intros.
+  * inversion H0; subst; try inversion H; try (proof_irr; auto).
+  * inversion H; subst. auto.
+  * inversion H0; subst; try inversion H'; try (proof_irr_many; auto).
+  * inversion H1; subst; try inversion H; auto.
+  * inversion H0; subst; try inversion H'; try (proof_irr_many; auto); try inversion_is_value.
+  * inversion H2; subst; try inversion_is_value; auto.
+  * inversion H0; subst; auto; try inversion H.
+  * inversion H1; subst; auto; try inversion_is_value.
+    rewrite H0 in H10. inversion H10. auto. congruence.
+  * inversion H2; subst; auto; try inversion_is_value. congruence.
+
+  * inversion H; subst; try inversion_is_value; try inversion H'; try inversion H1; try (proof_irr_many; auto).
+  * inversion H0; subst; try inversion_is_value. auto.
+  * inversion H1; subst; try inversion_is_value; auto.
+  * inversion H; subst; try inversion_is_value; try inversion H'; try inversion H1; try (proof_irr_many; auto).
+  * inversion H; subst; try congruence; try inversion_is_value; auto.
+  * inversion H; subst; try congruence; try inversion_is_value; auto.
+  * inversion H; subst; try congruence; try inversion_is_value; auto.
+  * inversion H; subst; try congruence; try inversion_is_value; auto.
+  * inversion H; subst; try congruence; try inversion_is_value; auto.
+Qed.
+
+Theorem value_nostep v (H : VALCLOSED v) :
+  forall fs' v', ⟨ [], v ⟩ --> ⟨fs' , v'⟩ -> False.
+Proof.
+  dependent induction H; intros.
+  * inversion H.
+  * inversion H.
+  * inversion H1.
+  * inversion H.
+  * inversion H.
+  * inversion H.
+  * inversion H0.
+Qed.
+
+Theorem step_rt_determinism {e v fs fs' k} :
+  ⟨fs, e⟩ -[k]-> ⟨fs', v⟩ -> VALCLOSED v
+->
+  (forall fs'' v', ⟨fs, e⟩ -[k]-> ⟨fs'', v'⟩ -> fs' = fs'' /\ v' = v).
+Proof.
+  intro. dependent induction H; intros.
+  * inversion H0; subst; auto.
+  * inversion H2; subst. apply IHstep_rt; auto. eapply step_determinism in H; eauto. destruct H. subst. auto.
+Qed.
+
+Theorem step_closedness : forall F e F' e',
+   ⟨ F, e ⟩ --> ⟨ F', e' ⟩ -> FSCLOSED F -> EXPCLOSED e
+->
+  FSCLOSED F' /\ EXPCLOSED e'.
+Proof.
+  intros F e F' e' IH. induction IH; intros; try inversion_is_value.
+  * inversion H0. subst. inversion H4. inversion H3. subst. split; auto.
+    constructor; auto. constructor; auto.
+  * inversion H. inversion H0. subst. split; auto. inversion H5. subst. cbn in H2.
+    apply -> subst_preserves_scope_exp; eauto.
+  * inversion H0. subst. inversion H5. inversion H9. subst. split; auto. constructor; auto.
+    constructor; auto.
+    apply Forall_app. split; auto.
+  * inversion H1. inversion H6. split. auto. subst. inversion H11.
+    apply -> subst_preserves_scope_exp; eauto. subst.
+    rewrite Nat.add_0_r. replace (S (length vl)) with (length (EFun vl e :: vs ++ [v])).
+    apply scoped_list_idsubst. constructor. auto. apply Forall_app. split; auto.
+    simpl. rewrite H0, app_length. simpl. lia.
+  * inversion H0. subst. inversion H4. inversion H3. subst. split; auto.
+    constructor; auto. constructor; auto.
+  * inversion H2. inversion H6. inversion H12.
+    subst. split; auto.
+    constructor; auto. constructor; auto.
+    apply Forall_app. split; auto.
+  * inversion H0. inversion H4. 
+    subst. split; auto. apply -> subst_preserves_scope_exp; eauto.
+  * inversion H1. inversion H5. subst. split; auto.
+    apply -> subst_preserves_scope_exp; eauto.
+    rewrite (match_pattern_length _ v l H0).
+    apply scoped_list_idsubst. eapply match_pattern_scoped; eauto.
+  * inversion H2. inversion H6. subst. split; auto.
+  * split; auto. inversion H0. 2: inversion H1. apply -> subst_preserves_scope_exp; eauto.
+  * inversion H0. inversion H4. subst. split; auto. repeat constructor; auto.
+  * inversion H1. inversion H5. subst. split; auto.
+  * inversion H; subst. split; auto.
+  * inversion H0. 2: inversion H1. subst. split; auto. constructor; auto.
+    now constructor.
+  * inversion H0. 2: inversion H1. subst. split; auto. constructor; auto.
+    constructor. rewrite indexed_to_forall. exact H4.
+  * inversion H0. 2: inversion H1. subst. split; auto. constructor; auto.
+    constructor. rewrite indexed_to_forall. exact H4.
+  * inversion H0. 2: inversion H1. subst. split; auto. constructor; auto.
+    constructor. rewrite Nat.add_0_r in H6. auto. auto.
+  * inversion H0; subst; split; auto. 1-2: constructor; auto; now constructor.
+    now inversion H1.
+Qed.
+
+Theorem result_VALCLOSED_any (fs : FrameStack) (e v : Exp) :
+  ⟨ fs, e ⟩ -->* v -> VALCLOSED v.
+Proof.
+  intros. destruct H. auto.
+Qed.
+
+Corollary step_any_closedness : forall F e v,
+   ⟨ F, e ⟩ -->* v -> FSCLOSED F -> EXPCLOSED e
+->
+  VALCLOSED v.
+Proof.
+  intros. destruct H, H2. induction H2.
+  * destruct e; try inversion H; now inversion H1.
+  * apply step_closedness in H2; auto.
+Qed.
+
+Definition terminates_sem (fs : FrameStack) (e : Exp) : Prop :=
+  exists v, ⟨fs, e⟩ -->* v.
+
+Definition terminates_in_k_sem (fs : FrameStack) (e : Exp) (k : nat) : Prop :=
+  exists v, ⟨fs, e⟩ -[k]-> ⟨[], v⟩ /\ VALCLOSED v.
+
+Open Scope nat_scope.
+
+(** Inductively defined termination relation. This will be used by the
+    equivalence concepts (CIU, CTX, logical relations).
+*)
+Reserved Notation "| fs , e | k ↓" (at level 80).
+Inductive terminates_in_k : FrameStack -> Exp -> nat -> Prop :=
+
+| term_value v : VALCLOSED v -> | [] , v | 0 ↓
+| term_case_true fs e1 e2 k v p l :
+  VALCLOSED v ->  match_pattern p v = Some l -> | fs , e1.[list_subst l idsubst] | k ↓
+ ->
+  | (FCase p e1 e2)::fs , v | S k ↓
+| term_case_false fs e1 e2 v k p :
+  VALCLOSED v ->  match_pattern p v = None -> | fs , e2 | k ↓ 
+ -> 
+  | (FCase p e1 e2)::fs , v | S k ↓
+| term_let_subst v e2 fs k x : VALCLOSED v -> | fs, e2.[v/] | k ↓ -> | (FLet x e2)::fs, v | S k ↓
+| term_letrec_subst vl b e fs f k : | fs, e.[EFun vl b/] | k ↓ -> | fs, ELetRec f vl b e | S k ↓
+| term_app_start v hd tl (H : VALCLOSED v) fs k : 
+  | (FApp2 v tl [])::fs, hd| k ↓ -> | (FApp1 (hd::tl))::fs, v | S k ↓
+| term_bif_start v hd tl (H : VALCLOSED v) fs k : 
+  | (FBIF2 v tl [])::fs, hd| k ↓ -> | (FBIF1 (hd::tl))::fs, v | S k ↓
+| term_app1 e fs k : | fs, e.[EFun [] e/] | k ↓ -> | (FApp1 [])::fs, EFun [] e | S k ↓
+| term_app_step v v' (H : VALCLOSED v) hd tl vs (H2 : Forall (fun v => VALCLOSED v) vs) (H' : VALCLOSED v') fs k :
+  | (FApp2 v tl (vs ++ [v']))::fs, hd | k ↓ -> | (FApp2 v (hd::tl) vs)::fs , v' | S k ↓
+| term_bif_step v v' (H : VALCLOSED v) hd tl vs (H2 : Forall (fun v => VALCLOSED v) vs) (H' : VALCLOSED v') fs k :
+  | (FBIF2 v tl (vs ++ [v']))::fs, hd | k ↓ -> | (FBIF2 v (hd::tl) vs)::fs , v' | S k ↓
+| term_plus (i1 i2 : Z) fs k :
+  | fs, ELit (Z.add i1 i2) | k ↓ ->
+  | (FBIF2 (ELit "+"%string) [] ([ELit (Int i1)]))::fs, ELit (Int i2) | S k ↓
+
+| term_app2 v vl e vs fs (H2 : Forall (fun v => VALCLOSED v) vs) k :
+  length vl = S (length vs) -> VALCLOSED v -> | fs, e.[list_subst (EFun vl e  :: (vs ++ [v])) idsubst] | k ↓ 
+-> | (FApp2 (EFun vl e) [] vs)::fs, v | S k ↓
+| term_cons1 e1 v2 fs k (H: VALCLOSED v2):
+  | FCons2 v2::fs, e1 | k ↓ -> | FCons1 e1 :: fs, v2 | S k ↓
+| term_cons2 v1 v2 fs k (H: VALCLOSED v2) (H0 : VALCLOSED v1):
+  | fs, VCons v1 v2 | k ↓ -> | FCons2 v2 :: fs, v1 | S k ↓
+
+| term_case e e1 e2 fs k p : | (FCase p e1 e2)::fs, e | k ↓ -> | fs, ECase e p e1 e2 | S k ↓
+| term_app e vs fs k : | (FApp1 vs)::fs, e | k ↓ -> | fs, EApp e vs | S k ↓
+| term_bif e vs fs k : | (FBIF1 vs)::fs, e | k ↓ -> | fs, EBIF e vs | S k ↓
+| term_let v e1 e2 fs k : | (FLet v e2)::fs, e1 | k ↓ -> | fs, ELet v e1 e2 | S k ↓
+| term_cons fs e1 e2 k :
+  | FCons1 e1 :: fs, e2 | k ↓ -> | fs, ECons e1 e2 | S k ↓
+where "| fs , e | k ↓" := (terminates_in_k fs e k).
+
+Definition terminates (fs : FrameStack) (e : Exp) := exists n, | fs, e | n ↓.
+Notation "| fs , e | ↓" := (terminates fs e) (at level 80).
+
+Theorem terminates_in_k_eq_terminates_in_k_sem :
+  forall k e fs, terminates_in_k_sem fs e k <-> | fs, e | k ↓.
+Proof.
+  induction k; intros.
+  * split; intros.
+    - inversion H. inversion H0. inversion H1. now constructor.
+    - inversion H. subst. econstructor. split. constructor. auto.
+  * split; intros.
+    {
+      inversion H. clear H. inversion H0; inversion H; subst.
+      assert (terminates_in_k_sem fs' e' k). { econstructor. eauto. } apply IHk in H2.
+      clear H0. inversion H3; subst.
+      1-7, 10-18: try econstructor; eauto.
+      * eapply term_case_true; eauto.
+      * apply term_case_false; auto.
+    }
+    {
+      inversion H; subst; clear H.
+      3-12: try match goal with
+      | [ H1 : | _, _ | _ ↓ |- _] => 
+         apply IHk in H1; destruct H1 as [e0 [H1e H1k]]; econstructor; split; 
+           [ econstructor; [ constructor | eauto ] | auto ]
+      end.
+      all : auto.
+      * apply IHk in H5. destruct H5, H.
+        econstructor; split. econstructor. constructor. all: eauto.
+      * apply IHk in H5. destruct H5, H.
+        econstructor; split. econstructor. apply red_case_false. all: eauto.
+      * apply IHk in H3. destruct H3, H.
+        econstructor; split. econstructor. constructor. eauto. auto.
+      * apply IHk in H3. destruct H3, H.
+        econstructor; split. econstructor. constructor. all: eauto.
+      * apply IHk in H6. destruct H6, H.
+        econstructor; split. econstructor. constructor. all: eauto.
+      * apply IHk in H5. destruct H5, H.
+        econstructor; split. econstructor. constructor. all: eauto.
+      * apply IHk in H3. destruct H3, H.
+        econstructor; split. econstructor. constructor. all: eauto.
+      * apply IHk in H3. destruct H3, H.
+        econstructor; split. econstructor. constructor. all: eauto.
+      * apply IHk in H3. destruct H3, H.
+        econstructor; split. econstructor. constructor. all: eauto.
+      * apply IHk in H3. destruct H3, H.
+        econstructor; split. econstructor. constructor. all: eauto.
+      * apply IHk in H3. destruct H3, H.
+        econstructor; split. econstructor. constructor. all: eauto.
+    }
+Qed.
+
+Corollary terminates_eq_terminates_sem :
+  forall e fs, terminates_sem fs e <-> | fs, e | ↓.
+Proof.
+  split; intros; inversion H.
+  * destruct H0, H1. econstructor. apply terminates_in_k_eq_terminates_in_k_sem.
+    econstructor. split; eauto.
+  * apply terminates_in_k_eq_terminates_in_k_sem in H0. destruct H0, H0. econstructor.
+    split. eauto. econstructor. eauto.
+Qed.
+
+Theorem terminates_step :
+  forall fs e, | fs, e | ↓ -> forall fs' e', ⟨fs, e⟩ --> ⟨fs', e'⟩
+->
+  | fs', e' | ↓.
+Proof.
+  intros. apply terminates_eq_terminates_sem in H. destruct H, H, H1. destruct x0.
+  * inversion H1. subst. apply value_nostep in H0; intuition.
+  * inversion H1. subst. apply (step_determinism H0) in H3. destruct H3. subst.
+    assert (terminates_sem fs' e'). { eexists. split. eauto. eexists. eauto. } apply terminates_eq_terminates_sem in H2.
+    auto.
+Qed.
+
+Theorem terminates_step_2 :
+  forall n fs e, | fs, e | n ↓ -> forall fs' e', ⟨fs, e⟩ --> ⟨fs', e'⟩
+->
+  | fs', e' | n - 1↓.
+Proof.
+  intros. apply terminates_in_k_eq_terminates_in_k_sem in H. destruct H. destruct n.
+  * destruct H. inversion H. subst. apply value_nostep in H0; intuition.
+  * destruct H.
+    inversion H. subst. apply (step_determinism H0) in H3. destruct H3. subst.
+    assert (exists y, ⟨ fs', e' ⟩ -[ n ]-> ⟨ [], y ⟩ /\ VALCLOSED y). { 
+      eexists. eauto. }
+    apply ex_intro in H6. apply terminates_in_k_eq_terminates_in_k_sem in H2.
+    now rewrite Nat.sub_1_r.
+Qed.
+
+Corollary terminates_step_any :
+  forall k fs e, | fs, e | ↓ -> forall fs' e', ⟨fs, e⟩ -[k]-> ⟨fs', e'⟩
+->
+  | fs', e' | ↓.
+Proof.
+  induction k; intros; inversion H0; subst; auto.
+  apply terminates_step in H2; auto. apply IHk in H5; auto.
+Qed.
+
+Corollary terminates_step_any_2 :
+  forall k n fs e, | fs, e | n ↓ -> forall fs' e', ⟨fs, e⟩ -[k]-> ⟨fs', e'⟩
+->
+  | fs', e' | n - k ↓.
+Proof.
+  induction k; intros; inversion H0; subst; auto.
+  * rewrite Nat.sub_0_r. auto.
+  * apply terminates_step_2 with (n := n) in H2; auto.
+    eapply IHk in H5; auto. 2: exact H2. now replace (n - S k) with ((n - 1) - k) by lia.
+Qed.
+
+Corollary transitive_eval : forall n  Fs Fs' e e',
+  ⟨ Fs, e ⟩ -[n]-> ⟨ Fs', e' ⟩ -> forall n' Fs'' e'', ⟨ Fs', e' ⟩ -[n']-> ⟨ Fs'', e'' ⟩
+->
+  ⟨ Fs, e ⟩ -[n + n']-> ⟨ Fs'', e''⟩.
+Proof.
+  intros n Fs F' e e' IH. induction IH; intros; auto.
+  simpl. econstructor. exact H. now apply IHIH.
+Qed.
+
+Corollary term_step_term :
+  forall k n fs e fs' e', ⟨fs, e⟩ -[k]-> ⟨fs', e'⟩ -> | fs', e' | n - k ↓ -> n >= k 
+->
+  | fs, e | n ↓.
+Proof.
+  intros. apply terminates_in_k_eq_terminates_in_k_sem.
+  apply terminates_in_k_eq_terminates_in_k_sem in H0. destruct H0, H0.
+  pose proof (transitive_eval _ _ _ _ _ H _ _ _ H0). replace (k+(n-k)) with n in H3 by lia.
+  eexists. eauto.
+Qed.
+
+Corollary term_step_term_plus :
+  forall k k2 fs e fs' e', 
+  ⟨fs, e⟩ -[k]-> ⟨fs', e'⟩ -> | fs', e' | k2 ↓
+->
+  | fs, e | k + k2 ↓.
+Proof.
+  intros. apply terminates_in_k_eq_terminates_in_k_sem.
+  apply terminates_in_k_eq_terminates_in_k_sem in H0. destruct H0, H0.
+  pose proof (transitive_eval _ _ _ _ _ H _ _ _ H0).
+  eexists. eauto.
+Qed.
+
+Lemma eval_app_partial :
+  forall vals vl e v Fs hds (P : VALCLOSED (EFun vl e)), length vl = length (hds ++ v :: vals) ->
+  Forall (fun v => VALCLOSED v) vals -> Forall (fun v => VALCLOSED v) hds -> VALCLOSED v ->
+  ⟨ FApp2 (EFun vl e) vals hds :: Fs, v ⟩ -[S (length vals)]-> ⟨ Fs , e.[list_subst (EFun vl e :: (hds ++ v :: vals)) idsubst]⟩.
+Proof.
+  induction vals; intros.
+  * simpl. econstructor. constructor; auto. rewrite app_length in H. simpl in H. lia.
+    constructor.
+  * simpl. econstructor. constructor; auto. inversion H0. subst.
+    epose proof (IHvals vl e a _ (hds ++ [v]) _ _ H6 _ H5). rewrite <- app_assoc in H3.
+    exact H3.
+  Unshelve.
+    auto.
+    rewrite <- app_assoc. auto. apply Forall_app. split. auto. constructor; auto.
+Qed.
+
+Lemma app1_eval :
+  forall vals Fs vl e (P : VALCLOSED (EFun vl e)), Forall (fun v => VALCLOSED v) vals -> length vl = length vals ->
+  exists k : nat,
+  ⟨ [FApp1 vals] ++ Fs, EFun vl e ⟩ -[ k ]-> ⟨ Fs, e.[EFun vl e .: list_subst vals idsubst] ⟩.
+Proof.
+  destruct vals; intros.
+  * apply length_zero_iff_nil in H0. subst. exists 1. econstructor.
+    simpl. constructor. cbn. constructor.
+  * exists (S (S (length vals))). simpl. econstructor. constructor. auto.
+    inversion H. subst.
+    apply eval_app_partial; auto.
+Qed.
+
+Lemma eval_app_partial_core :
+  forall hds' vals vl e e' v Fs hds (P : VALCLOSED (EFun vl e)),
+  Forall (fun v => VALCLOSED v) hds -> Forall (fun v => VALCLOSED v) hds' -> VALCLOSED v ->
+  ⟨ FApp2 (EFun vl e) (hds' ++ e' :: vals) hds :: Fs, v ⟩ -[S (length hds')]-> 
+  ⟨ FApp2 (EFun vl e) vals (hds ++ v :: hds') :: Fs , e'⟩.
+Proof.
+  induction hds'; intros.
+  * simpl. econstructor. constructor; auto. constructor.
+  * simpl. econstructor. constructor; auto. inversion H0. subst.
+    epose proof (IHhds' vals vl e _ a Fs (hds ++ [v]) _ _ _ H4).
+    rewrite <- app_assoc in H2. exact H2.
+  Unshelve.
+    auto.
+    apply Forall_app. split; auto. auto.
+Qed.
+
+Lemma full_eval_app_partial : forall e vals vl Fs (P : VALCLOSED (EFun vl e)),
+  length vl = length vals -> Forall (fun v => VALCLOSED v) vals ->
+  ⟨ Fs, EApp (EFun vl e) vals ⟩ -[2 + length vals]-> ⟨ Fs, e.[EFun vl e .: list_subst vals idsubst] ⟩.
+Proof.
+  destruct vals; intros.
+  - simpl. apply length_zero_iff_nil in H. subst. econstructor. constructor.
+    econstructor. constructor. constructor.
+  - simpl. econstructor. constructor.
+    econstructor. constructor. auto. inversion H0.
+    apply eval_app_partial; auto.
+Qed.
+
+Theorem transitive_eval_rev : forall Fs Fs' e e' k1,
+  ⟨ Fs, e ⟩ -[k1]-> ⟨ Fs', e' ⟩-> 
+  forall Fs'' e'' k2,
+  ⟨ Fs, e ⟩ -[k1 + k2]-> ⟨ Fs'', e'' ⟩
+->
+  ⟨ Fs', e' ⟩ -[k2]-> ⟨ Fs'', e'' ⟩.
+Proof.
+  intros Fs Fs' e e' k1 IH. induction IH; intros.
+  * simpl in H. auto.
+  * simpl in H0. inversion H0; subst. eapply step_determinism in H.
+    2: exact H2. destruct H; subst.
+    apply IHIH in H5. auto.
+Qed.
+
+Theorem app_term_fun : forall tl k hds e e' Fs (P : EXPCLOSED e)   (PP : Forall (fun v => EXPCLOSED v) tl),
+  | FApp2 e' tl hds :: Fs, e | k ↓ ->
+  Forall (fun v => VALCLOSED v) hds ->
+  (forall m : nat,
+    m < S k ->
+    forall (Fs : FrameStack) (e : Exp),
+    EXPCLOSED e -> | Fs, e | m ↓ ->
+    exists (v : Exp) (k : nat), VALCLOSED v /\ ⟨ Fs, e ⟩ -[ k ]-> ⟨ Fs, v ⟩)
+->
+  exists vl b, e' = EFun vl b /\ length vl = S (length (hds ++ tl)).
+Proof.
+  induction tl; intros.
+  * apply H1 in H as H'. 2: lia. destruct H', H2, H2.
+    eapply terminates_step_any_2 in H. 2: exact H3.
+    inversion H; subst; try inversion_is_value.
+    rewrite app_length, Nat.add_0_r. do 2 eexists. split. reflexivity. auto.
+    congruence.
+  * apply H1 in H as H'; auto. destruct H', H2, H2.
+    eapply terminates_step_any_2 in H. 2: exact H3.
+    inversion H; subst; try inversion_is_value.
+    apply H1 in H13 as H''. 2: lia. destruct H'', H4, H4.
+    eapply terminates_step_any_2 in H13. 2: exact H5.
+    apply IHtl in H13. destruct H13, H6, H6. subst. exists x3, x4. split; auto.
+    repeat rewrite app_length in *. simpl in *. lia.
+    3: apply Forall_app; auto.
+    2,4: inversion PP; auto.
+    constructor. auto.
+    intros. eapply H1. 3: exact H8. lia. auto.
+Qed.
+
+Theorem frame_indep_step : forall e F F' Fs e',
+  ⟨ F :: Fs, e ⟩ --> ⟨ F' :: Fs, e' ⟩
+->
+  forall Fs', ⟨ F :: Fs', e ⟩ --> ⟨ F' :: Fs', e' ⟩.
+Proof.
+  intros. revert Fs'. dependent induction H; intros.
+  all: try constructor; auto.
+  all: try (apply cons_neq in x; contradiction).
+  all: symmetry in x; try (apply cons_neq in x; contradiction).
+Qed.
+
+Theorem frame_indep_red : forall e F Fs e',
+  ⟨ F :: Fs, e ⟩ --> ⟨ Fs, e' ⟩
+->
+  forall Fs', ⟨ F :: Fs', e ⟩ --> ⟨ Fs', e' ⟩.
+Proof.
+  intros. revert Fs'. dependent induction H; intros.
+  all: try constructor; auto.
+  all: try (apply cons_neq in x; contradiction).
+  all: symmetry in x; try (apply cons_cons_neq in x; contradiction).
+Qed.
+
+Theorem frame_indep_core : forall k e Fs Fs' v,
+  ⟨ Fs, e ⟩ -[k]-> ⟨ Fs', v ⟩
+->
+  forall Fs'', ⟨ Fs ++ Fs'', e ⟩ -[k]-> ⟨ Fs' ++ Fs'', v ⟩.
+Proof.
+  induction k; intros.
+  * inversion H. subst. constructor.
+  * inversion H. subst. inversion H1; subst.
+    1-8, 10-18: simpl; econstructor; try constructor; auto.
+    all: try (eapply IHk in H4; simpl in H4; exact H4); auto.
+    econstructor. apply red_case_false; auto. apply IHk; auto.
+Qed.
+
+Theorem frame_indep_nil : forall k e Fs v,
+  ⟨ Fs, e ⟩ -[k]-> ⟨ [], v ⟩
+->
+  forall Fs', ⟨ Fs ++ Fs', e ⟩ -[k]-> ⟨ Fs', v ⟩.
+Proof.
+  intros. eapply frame_indep_core in H. exact H.
+Qed.
+
+Lemma term_app_length : forall tl hds e k Fs x0,
+  (forall m : nat,
+    m < S k ->
+    forall (Fs : FrameStack) (e : Exp),
+    | Fs, e | m ↓ ->
+    exists (v : Exp) (k : nat), VALCLOSED v /\ ⟨ Fs, e ⟩ -[ k ]-> ⟨ Fs, v ⟩ /\ k <= m) ->
+  | FApp2 x0 tl hds :: Fs, e | k ↓ -> k > length tl.
+Proof.
+  induction tl; intros.
+  * inversion H0; simpl; lia.
+  * simpl. apply H in H0 as H0'. destruct H0', H1, H1, H2.
+    eapply (terminates_step_any_2 _ _ _ _ H0) in H2 as H2'.
+    inversion H2'; subst; try inversion_is_value.
+    eapply IHtl in H13. lia. intros. apply H. lia. auto. lia.
+Qed.
+
+Lemma eval_app_partial_core_2 :
+  forall hds' vals vl e e' v Fs hds k (P : VALCLOSED (EFun vl e)) (PP : Forall (fun v => EXPCLOSED v) hds'),
+  (forall m : nat,
+    m < S k ->
+    forall (Fs : FrameStack) (e : Exp),
+    EXPCLOSED e -> | Fs, e | m ↓ ->
+    exists (v : Exp) (k : nat), VALCLOSED v /\ ⟨ Fs, e ⟩ -[ k ]-> ⟨ Fs, v ⟩) ->
+  | FApp2 (EFun vl e) (hds' ++ e' :: vals) hds :: Fs, v | k ↓ ->
+  VALCLOSED v ->
+  Forall (fun v => VALCLOSED v) hds ->
+  exists k0 hds'', k0 <= k /\ Forall (fun v => VALCLOSED v) hds'' /\
+  ⟨ FApp2 (EFun vl e) (hds' ++ e' :: vals) hds :: Fs, v ⟩ -[k0]-> 
+  ⟨ FApp2 (EFun vl e) vals (hds ++ v :: hds'') :: Fs , e'⟩.
+Proof.
+  induction hds'; intros.
+  * simpl in *. inversion H0; subst; try inversion_is_value.
+    exists 1, []. split. lia. split. auto. econstructor. constructor; auto. constructor.
+  * simpl in *. inversion H0; subst; try inversion_is_value.
+    apply H in H12 as P1. 2: lia. destruct P1, H3, H3.
+    eapply (terminates_step_any_2 _ _ _ _ H12) in H4 as H4'.
+    inversion H4'; subst; try inversion_is_value.
+    2: { destruct hds'; inversion H7. }
+    destruct hds'; simpl in H6; inversion H6; subst.
+    - simpl in H4.
+      assert (⟨ FApp2 (EFun vl e) (e' :: vals) (hds ++ [v]) :: Fs, x ⟩ -[1]->
+           ⟨ FApp2 (EFun vl e) vals ((hds ++ [v]) ++ [x]) :: Fs, e' ⟩).
+           { do 2 econstructor; auto. }
+      epose proof (transitive_eval _ _ _ _ _ H4 _ _ _ H5).
+      exists (S (x0 + 1)), [x]. split. lia. split. auto.
+      econstructor. constructor; auto.
+      rewrite <- app_assoc in H7. simpl in H7. auto.
+    - epose proof (IHhds' vals vl e e' x Fs _ _ _ _ _ H4' H'0 H15).
+      Unshelve. 4: { intros. eapply H. 3: exact H8. lia. auto. }
+      destruct H5, H5, H5, H7.
+      epose proof (transitive_eval _ _ _ _ _ H4 _ _ _ H8).
+      exists (S (x0 + x1)), (x::x2). 
+      split. 2: split.
+      + lia.
+      + constructor; auto.
+      + econstructor. constructor; auto. simpl in H9.
+        replace ((hds ++ [v]) ++ x :: x2) with (hds ++ v :: x :: x2) in H9.
+        exact H9.
+        rewrite <- app_assoc. auto.
+      + auto.
+      + now inversion PP.
+    - now inversion PP.
+Qed.
+
+Lemma eval_app_partial_core_emtpy :
+  forall hds' vals vfun e' v Fs hds k (P : VALCLOSED vfun) (PP : Forall (fun v => EXPCLOSED v) hds'),
+  (forall m : nat,
+    m < S k ->
+    forall (Fs : FrameStack) (e : Exp),
+    EXPCLOSED e -> | Fs, e | m ↓ 
+    -> exists (v : Exp) (k : nat), VALCLOSED v /\ ⟨ [], e ⟩ -[ k ]-> ⟨ [], v ⟩) ->
+  | FApp2 vfun (hds' ++ e' :: vals) hds :: Fs, v | k ↓ ->
+  VALCLOSED v ->
+  Forall (fun v => VALCLOSED v) hds ->
+  exists k0 hds'', k0 <= k /\ Forall (fun v => VALCLOSED v) hds'' /\
+  ⟨ [FApp2 vfun (hds' ++ e' :: vals) hds], v ⟩ -[k0]-> 
+  ⟨ [FApp2 vfun vals (hds ++ v :: hds'')] , e'⟩.
+Proof.
+  induction hds'; intros.
+  * simpl in *. inversion H0; subst; try inversion_is_value.
+    exists 1, []. split. lia. split. auto. econstructor. constructor; auto. constructor.
+  * simpl in *. inversion H0; subst; try inversion_is_value.
+    apply H in H12 as P1. 2: lia. destruct P1, H3, H3.
+    eapply frame_indep_nil in H4 as H4_1.
+    eapply (terminates_step_any_2 _ _ _ _ H12) in H4_1 as H4'.
+    inversion H4'; subst; try inversion_is_value.
+    2: { destruct hds'; inversion H6. }
+    destruct hds'; simpl in H6; inversion H6; subst.
+    - simpl in H4.
+      assert (⟨ [FApp2 vfun (e' :: vals) (hds ++ [v])], x ⟩ -[1]->
+           ⟨ [FApp2 vfun vals ((hds ++ [v]) ++ [x])], e' ⟩).
+           { do 2 econstructor; auto. }
+      eapply frame_indep_nil in H4.
+      epose proof (transitive_eval _ _ _ _ _ H4 _ _ _ H5).
+      exists (S (x0 + 1)), [x]. split. lia. split. auto.
+      econstructor. constructor; auto.
+      rewrite <- app_assoc in H7. simpl in H7. auto.
+    - epose proof (IHhds' vals vfun e' x Fs _ _ _ _ _ H4' H'0 H15).
+      Unshelve. 4: { intros. eapply H. 3: exact H8. lia. auto. }
+      destruct H5, H5, H5, H7.
+      eapply frame_indep_nil in H4.
+      epose proof (transitive_eval _ _ _ _ _ H4 _ _ _ H8).
+      exists (S (x0 + x1)), (x::x2). 
+      split. 2: split.
+      + lia.
+      + constructor; auto.
+      + econstructor. constructor; auto. simpl in H9.
+        replace ((hds ++ [v]) ++ x :: x2) with (hds ++ v :: x :: x2) in H9.
+        exact H9.
+        rewrite <- app_assoc. auto.
+      + auto.
+      + now inversion PP.
+    - now inversion PP.
+Qed.
+
+Lemma term_bif_eval_empty :
+  forall tl Fs v0 vals lst hd k,
+  (forall m : nat,
+    m < S k ->
+    forall (Fs : FrameStack) (e : Exp),
+    EXPCLOSED e ->
+    | Fs, e | m ↓ ->
+    exists (v : Exp) (k : nat),
+      VALCLOSED v /\
+      ⟨ [], e ⟩ -[ k ]-> ⟨ [], v ⟩) ->
+  | FBIF2 v0 (tl ++ [lst]) vals :: Fs, hd | k ↓ ->
+  VALCLOSED hd ->
+  Forall (fun e => EXPCLOSED e) tl ->
+  Forall (fun e => VALCLOSED e) vals ->
+  exists i vals', i <= k /\ Forall (fun v => VALCLOSED v) vals' /\
+    ⟨ FBIF2 v0 (tl ++ [lst]) vals :: [], hd ⟩ -[i]->
+    ⟨ FBIF2 v0 [] (vals ++ [hd] ++ vals') :: [], lst ⟩.
+Proof.
+  induction tl; intros; simpl.
+  * inversion H0; subst; try inversion_is_value.
+    exists 1, []. split. 2: split. 2: auto.
+    lia.
+    econstructor. constructor; auto. constructor.
+  * inversion H2; subst.
+    inversion H0; subst; try inversion_is_value.
+    apply H in H15 as HH; auto. destruct HH as [v1 [k1 [v1cl HH]]].
+    eapply frame_indep_nil in HH as HH0.
+    eapply (terminates_step_any_2 _ _ _ _ H15) in HH0 as HH'; auto.
+    destruct (k0 - k1) eqn:Eq. inversion HH'.
+    epose proof (IHtl Fs v0 (vals ++ [hd]) lst v1 (S n) _ HH' v1cl H7 _).
+    destruct H4 as [k2 [vals' [Hlt [Fcl H4]]]].
+    exists (S (k1 + k2)), (v1 :: vals').
+    split. 2: split. lia.
+    constructor; auto.
+    econstructor. constructor; auto.
+    eapply transitive_eval.
+    eapply frame_indep_nil in HH. exact HH.
+    simpl in H4.
+    rewrite <- app_assoc in H4. exact H4.
+  Unshelve.
+    intros. eapply H. 3: exact H8. lia. auto. apply Forall_app; auto.
+Qed.
+
+(* NOTE: This is not a duplicate! Do not remove! *)
+Theorem term_eval_empty : forall x Fs e (P : EXPCLOSED e), | Fs, e | x ↓ ->
+  exists v k, VALCLOSED v /\ ⟨ [], e ⟩ -[k]-> ⟨ [], v ⟩ (* /\ k <= x *).
+Proof.
+  induction x using lt_wf_ind. destruct x; intros; inversion H0; subst; try congruence.
+  * exists e, 0. now repeat constructor.
+  * exists e, 0. split; [ auto | do 2 constructor ].
+  * exists e, 0. split; [ auto | now constructor ].
+  * exists e, 0. split; [ auto | now constructor].
+  * apply H in H4. destruct H4, H1, H1. exists x0, (S x1).
+    split; [ auto | ]. econstructor. constructor. auto. lia.
+    inversion P. 2: inversion_is_value. apply -> subst_preserves_scope_exp; eauto.
+  * exists e, 0. split; [ auto | now constructor ].
+  * exists e, 0. split; [ auto | now constructor ].
+  * exists (EFun [] e0), 0. inversion P. split; [ auto | do 2 constructor].
+  * exists e, 0. split; [ auto | now constructor].
+  * exists e, 0. split; [ auto | now constructor ].
+  * exists (ELit i2), 0. split; [ auto | now constructor ].
+  * exists e, 0. split; [ auto | now constructor ].
+  * exists e, 0. split; [ auto | now constructor ].
+  * exists e, 0. split; [ auto | now constructor ].
+  * apply H in H4 as HH. destruct HH, H1, H1. 2: lia.
+    eapply frame_indep_nil in H2 as H2_1.
+    eapply (terminates_step_any_2 _ _ _ _ H4) in H2_1 as H2'.
+    inversion H2'; subst; try inversion_is_value.
+    - apply H in H12. 2: lia. destruct H12, H3, H3.
+      exists x2, (S (x1 + S x3)). split. auto.
+      econstructor. constructor. eapply transitive_eval; eauto.
+      eapply frame_indep_nil in H2. exact H2.
+      econstructor. constructor. all: eauto. inversion P. 2: inversion_is_value.
+      subst. apply -> subst_preserves_scope_exp. exact H13.
+      rewrite (match_pattern_length _ _ _ H11), Nat.add_0_r.
+      eapply scoped_list_idsubst, match_pattern_scoped. exact H9. eauto.
+    - apply H in H12. 2: lia. destruct H12, H3, H3.
+      exists x2, (S (x1 + S x3)). split. auto.
+      econstructor. constructor. eapply transitive_eval; eauto.
+      eapply frame_indep_nil in H2. exact H2.
+      econstructor. apply red_case_false; auto. auto. now inversion P.
+    - now inversion P.
+  * apply H in H4 as v_eval. 2: lia. destruct v_eval, H1, H1.
+    eapply frame_indep_nil in H2 as H2_1.
+    eapply (terminates_step_any_2 _ _ _ _ H4) in H2_1 as H2'.
+    destruct vs.
+    - inversion H2'; subst; try inversion_is_value.
+      apply H in H7. 2: lia. destruct H7, H3, H3.
+      exists x0, (S (x1 + S x2)). split; auto.
+      econstructor. constructor. eapply transitive_eval; eauto.
+      eapply frame_indep_nil in H2. exact H2.
+      econstructor. constructor. auto.
+      inversion H1. apply -> subst_preserves_scope_exp; eauto.
+    - inversion H2'; subst; try inversion_is_value.
+      assert (| FApp2 x0 vs [] :: Fs, e | k ↓) as PP by auto.
+      eapply H in H10. 2: lia. destruct H10, H3, H3.
+      destruct (length vs) eqn:P0.
+      + apply length_zero_iff_nil in P0. subst.
+        eapply frame_indep_nil in H5 as H5_1.
+        eapply (terminates_step_any_2 _ _ _ _ PP) in H5_1 as H5'.
+        inversion H5'; subst; try inversion_is_value.
+        apply H in H16. 2: lia. destruct H16, H6, H6.
+        assert (⟨ [FApp2 (EFun vl e1) [] []], x2 ⟩ -[1]-> ⟨ [], e1.[list_subst (EFun vl e1 :: [] ++ [x2]) idsubst] ⟩).
+        { repeat econstructor; auto. }
+        eapply frame_indep_nil in H7.
+        epose proof (transitive_eval _ _ _ _ _ H10 _ _ _ H7).
+        assert (⟨ [FApp1 [e]], EFun vl e1 ⟩ -[1]-> ⟨ [FApp2 (EFun vl e1) [] []], e ⟩). { do 2 econstructor; auto. }
+        eapply frame_indep_nil in H2.
+        epose proof (transitive_eval _ _ _ _ _ H2 _ _ _ H16).
+        eapply frame_indep_nil in H5.
+        epose proof (transitive_eval _ _ _ _ _ H5 _ _ _ H10).
+        epose proof (transitive_eval _ _ _ _ _ H17 _ _ _ H18).
+        epose proof (transitive_eval _ _ _ _ _ H19 _ _ _ H7).
+        exists x0, (S (x1 + 1 + (x3 + 1) + x4)). split; auto.
+        econstructor. constructor. auto.
+        inversion H1.
+        apply -> subst_preserves_scope_exp; eauto; subst.
+        simpl. apply cons_scope; auto. rewrite H14. apply cons_scope; auto.
+      + apply eq_sym, last_element_exists in P0. destruct P0, H6. subst.
+        eapply frame_indep_nil in H5 as H5_1.
+        eapply (terminates_step_any_2 _ _ _ _ PP) in H5_1 as H5'.
+
+        epose proof (eval_app_partial_core_emtpy x4 [] x0 x5 _ _ _ _ _ _ _ H5' H3 ltac:(auto)).
+        destruct H6, H6, H6, H7. simpl in H10.
+        eapply frame_indep_core in H10 as H10_1. simpl in H10_1.
+        eapply (terminates_step_any_2 _ _ _ _ H5') in H10_1 as H7'.
+        apply H in H7' as H7''. 2: lia. destruct H7'', H11, H11.
+        eapply frame_indep_nil in H12 as H12_1.
+        eapply (terminates_step_any_2 _ _ _ _ H7') in H12_1 as H11'.
+        inversion H11'; subst; try inversion_is_value.
+        apply H in H21. 2: lia. destruct H21, H13, H13.
+        eapply frame_indep_nil in H12.
+        epose proof (transitive_eval _ _ _ _ _ H10 _ _ _ H12).
+        assert (⟨ [FApp2 (EFun vl e1) [] (x2 :: x7)], x8 ⟩ -[1]->
+              ⟨ [], e1.[list_subst (EFun vl e1 :: (x2 :: x7) ++ [x8]) idsubst] ⟩). { econstructor. constructor; auto. constructor. }
+        epose proof (transitive_eval _ _ _ _ _ H15 _ _ _ H18).
+        epose proof (transitive_eval _ _ _ _ _ H21 _ _ _ H14).
+        eapply frame_indep_nil in H5.
+        epose proof (transitive_eval _ _ _ _ _ H5 _ _ _ H22).
+        assert (⟨ [FApp1 (e :: x4 ++ [x5])], EFun vl e1 ⟩ -[1]->
+            ⟨ [FApp2 (EFun vl e1) (x4 ++ [x5]) []] , e ⟩).
+            { econstructor. constructor. auto. constructor. }
+        simpl app in *.
+        epose proof (transitive_eval _ _ _ _ _ H24 _ _ _ H23).
+        eapply frame_indep_nil in H2.
+        epose proof (transitive_eval _ _ _ _ _ H2 _ _ _ H25).
+
+        exists x0, (S (x1 + (1 + (x3 + (x6 + x9 + 1 + x10))))). split; auto.
+        econstructor. constructor. auto.
+     Unshelve.
+       ** inversion H1. subst. apply -> subst_preserves_scope_exp; eauto.
+          replace (S (Datatypes.length vl) + 0) with (length ((EFun vl e1 :: (x2 :: x7) ++ [x8]))). 2: { simpl. rewrite app_length. simpl in *. lia. }
+          apply scoped_list_idsubst. simpl. do 2 constructor; auto.
+          apply Forall_app; auto.
+        ** inversion P. 2: inversion_is_value.
+           subst. rewrite <- indexed_to_forall in H14.
+           inversion H14. subst. rewrite Forall_app in H16; auto.
+           destruct H16. now inversion H12.
+        ** inversion P. 2: inversion_is_value.
+           rewrite <- indexed_to_forall in H11. now inversion H11.
+        ** inversion P. 2: inversion_is_value.
+           rewrite <- indexed_to_forall in H11. inversion H11.
+           now rewrite Forall_app in H15.
+        ** intros. eapply H. 3: exact H10. lia. auto.
+      + inversion P. 2: inversion_is_value. apply (H7 0); simpl; lia.
+    - now inversion P.
+  * inversion P; subst. 2: inversion_is_value.
+    apply H in H4 as HH; auto. destruct HH as [v0 [k0 [v0CL HH]]].
+    eapply frame_indep_nil in HH as HH0.
+    eapply (terminates_step_any_2 _ _ _ _ H4) in HH0 as HH'.
+    inversion HH'; subst; try inversion_is_value; auto.
+    destruct (length tl) eqn:Len.
+    - apply length_zero_iff_nil in Len. subst.
+      apply H in H9 as H9'; auto. 2: lia.
+      destruct H9' as [hd' [k1 [hd'Vcl H9']]].
+      eapply frame_indep_nil in H9' as H9'0.
+      eapply (terminates_step_any_2 _ _ _ _ H9) in H9'0 as H9''.
+      inversion H9''; subst; try inversion_is_value.
+      inversion P; subst. apply (H10 0 ltac:(simpl;lia)).
+      inversion_is_value.
+    - apply eq_sym, last_element_exists in Len as [tl' [lst ?]]; subst.
+      inversion P; subst; try inversion_is_value.
+      apply indexed_to_forall in H10.
+      inversion H10. subst. apply Forall_app in H12 as [H12_1 H12_2].
+      inversion H12_2; subst.
+      apply H in H9 as H9'; auto. 2: lia.
+      destruct H9' as [hd' [k1 [hd'Vcl H9']]].
+      eapply frame_indep_nil in H9' as H9'0.
+      eapply (terminates_step_any_2 _ _ _ _ H9) in H9'0 as H9''.
+      epose proof (term_bif_eval_empty tl' Fs v0 [] lst hd' _ _ H9'' _ _ _).
+      destruct H1 as [k2 [vals' [Hlt [Hall Der]]]].
+      eapply frame_indep_core in Der as Der0.
+      eapply (terminates_step_any_2 _ _ _ _ H9'') in Der0 as Der'.
+      eapply H in Der' as Der''; auto. 2: lia.
+      destruct Der'' as [lstval [k3 [VCl3 Der'']]].
+      eapply frame_indep_nil in Der'' as Der''0.
+      epose proof (transitive_eval _ _ _ _ _ Der _ _ _ Der''0) as DEND.
+      simpl app in *.
+      eapply frame_indep_nil in H9'.
+      epose proof (transitive_eval _ _ _ _ _ H9' _ _ _ DEND) as COMP.
+      assert (⟨ FBIF1 (hd :: tl' ++ [lst]) :: [], v0 ⟩ -[1]->
+              ⟨ FBIF2 v0 (tl' ++ [lst]) [] :: [], hd ⟩) as ONE. {
+        econstructor. constructor. auto. constructor.
+      }
+      epose proof (transitive_eval _ _ _ _ _ ONE _ _ _ COMP) as COMP'.
+      eapply frame_indep_nil in HH.
+      epose proof (transitive_eval _ _ _ _ _ HH _ _ _ COMP') as COMP''.
+      simpl in COMP''.
+      eapply frame_indep_nil in Der''.
+      eapply (terminates_step_any_2 _ _ _ _ Der') in Der'' as Der'''.
+      inversion Der'''; subst; try inversion_is_value.
+      exists (ELit (i1 + i2)%Z). eexists.
+      split; auto.
+      econstructor. constructor.
+      eapply transitive_eval. exact COMP''.
+      econstructor. constructor. constructor.
+    Unshelve.
+      all: auto.
+      intros. eapply H. 3: exact H14. lia. auto.
+  * apply H in H4 as HH. destruct HH, H1, H1. 2: lia.
+    eapply frame_indep_nil in H2 as H2_1.
+    eapply (terminates_step_any_2 _ _ _ _ H4) in H2_1 as H2'.
+    inversion H2'; subst; try inversion_is_value.
+    apply H in H10 as HH. destruct HH, H3, H3. 2: lia.
+    eapply frame_indep_nil in H5 as H5_1.
+    eapply (terminates_step_any_2 _ _ _ _ H10) in H5_1 as H5'.
+    exists x2, (S (x1 + (S x3))).
+    split. auto.
+    econstructor. constructor. eapply transitive_eval; eauto.
+    eapply frame_indep_nil in H2. exact H2. 
+    econstructor. constructor; auto. auto.
+
+    inversion P. 2: inversion_is_value. 
+    apply -> subst_preserves_scope_exp; eauto.
+    now inversion P.
+  * apply H in H4 as HH. 2: lia. 2: now inversion P.
+    destruct HH as [v2 [k2 [V2CL Eval2]]].
+    eapply frame_indep_nil in Eval2 as Eval2'.
+    eapply (terminates_step_any_2 _ _ _ _ H4) in Eval2'.
+    inversion Eval2'; subst; try inversion_is_value.
+    apply H in H7 as [v1 [k1 [V1CL Eval1]]]. 2: lia. 2: now inversion P.
+    assert (⟨ [FCons1 e1], v2 ⟩ -[1]-> ⟨ [FCons2 v2], e1 ⟩).
+    { econstructor. constructor. auto. constructor. }
+    eapply transitive_eval in H1.
+    2: eapply frame_indep_nil in Eval2 as Eval2''; exact Eval2''.
+    eapply frame_indep_nil in Eval1 as Eval1''.
+    eapply transitive_eval in Eval1''. 2: exact H1.
+    assert (⟨ [FCons2 v2], v1 ⟩ -[1]-> ⟨ [], VCons v1 v2 ⟩).
+    { econstructor. constructor; auto. constructor. }
+    eapply transitive_eval in H2. 2: exact Eval1''.
+    exists (VCons v1 v2), (S ((k2 + 1 + k1) + 1)). split. constructor; auto.
+    econstructor. constructor; auto. exact H2.
+Qed.
+
+Corollary term_eval : forall x Fs e (P : EXPCLOSED e), | Fs, e | x ↓ ->
+  exists v k, VALCLOSED v /\ ⟨ Fs, e ⟩ -[k]-> ⟨ Fs, v ⟩ (* /\ k <= x *).
+Proof.
+  intros.
+  pose proof (term_eval_empty x Fs e P H).
+  destruct H0, H0, H0.
+  do 2 eexists. split; eauto. eapply frame_indep_nil in H1. exact H1.
+Qed.
+
+Corollary app_term_fun_final : forall tl k hds e e' Fs,
+  | FApp2 e' tl hds :: Fs, e | k ↓ -> Forall (fun v => VALCLOSED v) hds ->
+  EXPCLOSED e -> Forall (fun e => EXPCLOSED e) tl
+->
+  exists vl b, e' = EFun vl b /\ length vl = S (length (hds ++ tl)).
+Proof.
+  intros. eapply app_term_fun; eauto.
+  intros. eapply term_eval. eauto. eauto.
+Qed.
+
+Corollary term_eval_both : forall x Fs e (P : EXPCLOSED e), | Fs, e | x ↓ ->
+  exists v k, VALCLOSED v /\ ⟨ [], e ⟩ -[k]-> ⟨ [], v ⟩ /\ ⟨ Fs, e ⟩ -[k]-> ⟨ Fs, v ⟩.
+Proof.
+  intros. apply term_eval_empty in H. destruct H, H, H.
+  exists x0, x1; split; [| split]; auto.
+  eapply frame_indep_nil in H0; eauto. auto.
+Qed.
+
+Theorem app_term_conditions : forall l1 l2 v e x Fs (P : EXPCLOSED e) (PP : Forall (fun e => EXPCLOSED e) l1), 
+  | FApp2 v l1 l2 :: Fs, e | x ↓ ->
+  Forall (fun v => VALCLOSED v) l2 /\ exists vl e', v = EFun vl e'.
+Proof.
+  induction l1; intros.
+  * apply term_eval in H as H'; auto. destruct H', H0, H0.
+    eapply (terminates_step_any_2 _ _ _ _ H) in H1 as H1'.
+    inversion H1'; subst; try inversion_is_value. split. auto. now do 2 eexists.
+  * apply term_eval in H as H'. destruct H', H0, H0.
+    eapply (terminates_step_any_2 _ _ _ _ H) in H1 as H1'.
+    inversion H1'; subst; try inversion_is_value. apply IHl1 in H11.
+    destruct H11, H3, H3. split; auto. subst. now do 2 eexists.
+    now inversion PP.
+    now inversion PP.
+    congruence.
+Qed.
+
+Lemma eval_bif_partial :
+  forall hds vals vfun v Fs,
+  Forall (fun v => EXPCLOSED v) vals ->
+  Forall (fun v => VALCLOSED v) hds ->
+  VALCLOSED vfun ->
+  EXPCLOSED v ->
+  ⟨ Fs, EBIF vfun (hds ++ v :: vals) ⟩ -[S (S (length hds))]-> 
+  ⟨ FBIF2 vfun vals hds :: Fs , v⟩.
+Proof.
+  intro hds.
+  remember (length hds) as len. generalize dependent hds.
+  induction len; intros.
+  * apply eq_sym, length_zero_iff_nil in Heqlen. subst.
+    simpl. econstructor. constructor; auto.
+    econstructor. constructor; auto. constructor.
+  * apply last_element_exists in Heqlen as L'.
+    destruct L' as [hds' [lst Eq]]; subst.
+    apply Forall_app in H0 as [H0_1 H0_2]. inversion H0_2; subst.
+    rewrite app_length in Heqlen. simpl in Heqlen.
+    specialize (IHlen hds' ltac:(lia) (v::vals) vfun lst Fs
+         ltac:(constructor;auto) H0_1 H1 ltac:(constructor;auto)).
+    rewrite <- app_assoc. simpl.
+    replace (S (S (S len))) with (S (S len) + 1) by lia.
+    eapply transitive_eval. exact IHlen.
+    econstructor. constructor; auto. constructor.
+Qed.
+
+Theorem put_back : forall F e Fs (P : EXPCLOSED e) (P2 : FCLOSED F),
+  | F :: Fs, e | ↓ -> | Fs, plug_f F e | ↓.
+Proof.
+  destruct F; intros; simpl.
+  * inversion H. exists (S x). constructor. auto.
+  * destruct H.
+    apply term_eval in H as H'. destruct H', H0, H0.
+    apply app_term_conditions in H as CDS. destruct CDS, H3, H3. subst.
+    destruct l2.
+    - simpl in *. exists (2 + x). do 2 constructor; auto.
+      now inversion P2.
+    - inversion H2. subst.
+      epose proof (eval_app_partial_core l2 l1 x2 x3 e e0 Fs [] _ _ H6 H5).
+      exists (2 + (S (Datatypes.length l2) + x)). simpl.
+      do 2 constructor. now inversion P2.
+      apply terminates_in_k_eq_terminates_in_k_sem in H.
+      apply terminates_in_k_eq_terminates_in_k_sem. destruct H, H.
+      exists x4. split; auto. rewrite <- Nat.add_succ_l.
+      eapply transitive_eval. exact H3. auto.
+    - auto.
+    - now inversion P2.
+    - auto.
+  * inversion H. exists (S x). constructor. auto.
+  * inversion H. exists (S x). constructor. auto.
+  * inversion H. exists (S x). constructor. auto.
+  * inversion H. exists (S (S x)). inversion P2. do 2 constructor; auto.
+  * destruct H. exists (S x). constructor. auto.
+  * destruct H. 
+    apply term_eval in H as HH; auto.
+    destruct HH as [? [? [? ?]]]. inversion P2; subst.
+    pose proof (eval_bif_partial l2 l1 v e Fs H6 H7 H5 P).
+    eexists.
+    eapply term_step_term_plus. exact H2. exact H.
+Unshelve.
+  now inversion P2.
+  auto.
+Qed.
+
+Theorem put_back_rev : forall F e Fs (P : EXPCLOSED e), FCLOSED F ->
+  | Fs, plug_f F e | ↓ -> | F :: Fs, e | ↓.
+Proof.
+  destruct F; intros; simpl.
+  * destruct H0. simpl in H0. inversion H0; subst; try inversion_is_value. eexists. eauto.
+  * simpl in *. inversion H. subst. destruct H0.
+    destruct l2.
+    - simpl in H0. inversion H0; subst; try inversion_is_value.
+      inversion H8; subst; try inversion_is_value. eexists. eauto.
+    - inversion H0; subst; try inversion_is_value.
+      inversion H8; subst; try inversion_is_value.
+      inversion H6; subst.
+      apply app_term_conditions in H11 as COND.
+      2: now constructor.
+      2: apply Forall_app; split; [ | constructor]; auto.
+      destruct COND as [FC [vl [b ?]]]. subst.
+      epose proof (eval_app_partial_core l2 l1 vl b e e0 Fs [] ltac:(auto) ltac:(auto) H7 H3).
+      simpl in H1.
+      eapply (terminates_step_any_2 _ _ _ _ H11) in H1 as H1'. eexists. exact H1'.
+      eapply Forall_impl. 2: exact H7. intros. now constructor.
+  * destruct H0. simpl in H0. inversion H0; subst; try inversion_is_value. eexists. eauto.
+  * destruct H0. simpl in H0. inversion H0; subst; try inversion_is_value. eexists. eauto.
+  * destruct H0. simpl in H0. inversion H0; subst; try inversion_is_value. eexists. eauto.
+  * destruct H0. simpl in H0. inversion H0; subst; try inversion_is_value. inversion H.
+    subst. inversion H5; subst; try inversion_is_value. eexists. eauto.
+  * destruct H0. simpl in H0. inversion H0; subst; try inversion_is_value. eexists. eauto.
+  * simpl in H0. inversion H. subst. 
+    destruct H0.
+    pose proof (eval_bif_partial l2 l1 v e Fs H5 H6 H4 P).
+    eexists.
+    eapply terminates_step_any_2. exact H0.
+    exact H1.
+Qed.
+
+Theorem term_app_in_k : forall Fs vl vals e k (P : VALCLOSED (EFun vl e)),
+  length vl = length vals -> Forall (fun v => VALCLOSED v) vals ->
+  | Fs, e.[EFun vl e .: list_subst vals idsubst] | k ↓ ->
+  | Fs, EApp (EFun vl e) vals | 2 + length vl + k ↓.
+Proof.
+  intros. inversion H0; try inversion_is_value; subst.
+  * apply length_zero_iff_nil in H. subst.
+    do 2 constructor. auto.
+  * destruct (length l) eqn:D1.
+    - apply length_zero_iff_nil in D1. subst. rewrite H. simpl.
+      do 2 constructor; auto. now constructor.
+    - apply eq_sym, last_element_exists in D1 as D1'. destruct D1' as [l' [l'x EQ]].
+      subst. apply Forall_app in H3 as [H3_1 H3_2]. inversion H3_2. subst.
+      epose proof (eval_app_partial_core l' [] vl e l'x x Fs []
+         ltac:(constructor) _ H3_1 H2). cbn in H3.
+      assert (⟨ FApp2 (EFun vl e) [] (x :: l') :: Fs, l'x ⟩ -[1]-> ⟨ Fs, e.[EFun vl e .: list_subst (x :: l' ++ [l'x]) idsubst] ⟩). { 
+        econstructor; constructor. all: auto.
+        simpl. simpl in H. rewrite app_length in H. simpl in H. lia.
+      }
+      epose proof (transitive_eval _ _ _ _ _ H3 _ _ _ H4).
+      eapply term_step_term_plus in H7. 2: exact H1.
+      rewrite H. simpl. rewrite app_length. simpl. do 2 constructor. auto. exact H7.
+  Unshelve.
+    now inversion P.
+    auto.
+Qed.
+
+(** The following two theorems state general properties about the evaluation
+    of map and foldr. Specifically, they explain the conditions under they
+    evaluate to the same list value. *)
+Theorem obj_map_on_meta_level :
+  forall l' l x e f
+  (VsCL : VALCLOSED l) (SCE : EXP 2 ⊢ e),
+  computes x e f -> cons_to_list l = Some l' ->
+  ⟨[], obj_map (EFun [x] e) l⟩ -->* list_to_cons (map f l').
+Proof.
+  induction l'; intros.
+  * destruct l; simpl in H0; inversion H0.
+    2: { destruct (cons_to_list l2); inversion H0. }
+    unfold obj_map. cbn.
+    eexists. auto. eexists.
+    econstructor. constructor. cbn.
+    econstructor. constructor.
+    econstructor. constructor. {
+      constructor. simpl. constructor; auto.
+      cbn. do 2 constructor; auto. 2: do 2 constructor; lia.
+      all: intros; destruct i; simpl; constructor; auto; simpl in *.
+      2-3: destruct i; try constructor; lia. constructor. lia.
+    }
+    econstructor. constructor. {
+      constructor. simpl. constructor; auto.
+      cbn. do 2 constructor; auto. 2: do 2 constructor; lia.
+      all: intros; destruct i; simpl; constructor; auto; simpl in *.
+      2-3: destruct i; try constructor; lia. constructor. lia.
+    } auto.
+    {
+      constructor. simpl. rewrite (proj2 (scoped_ignores_sub 2) e); auto.
+    }
+    simpl.
+    econstructor. constructor; auto. constructor; auto.
+    {
+      constructor. simpl. rewrite (proj2 (scoped_ignores_sub 2) e); auto.
+    }
+    econstructor. simpl. constructor; auto. cbn.
+    econstructor. apply red_case_false; auto.
+    constructor.
+  * destruct l; simpl in H0; inversion H0.
+    break_match_hyp; inversion H0. subst.
+    inversion VsCL. subst.
+    clear H0 H2 VsCL. specialize (IHl' _ _ _ _  H5 SCE H Heqo).
+    destruct IHl' as [VCL [k H']].
+    unfold obj_map in H'. inversion H'; subst.
+    1: { rewrite <- H3 in VCL. inversion_is_value. } clear H'.
+    inversion H0; subst. clear H0. simpl in H1.
+    (** eval first element (necessary before eexists): *)
+    specialize (H a) as [? [kk DER]].
+    (***)
+    unfold obj_map. split. { simpl. constructor; auto. }
+
+    eexists.
+    econstructor. constructor. cbn.
+    econstructor. constructor.
+    econstructor. constructor. {
+      constructor. simpl. constructor; auto.
+      cbn. do 2 constructor; auto. 2: do 2 constructor; lia.
+      all: intros; destruct i; simpl; constructor; auto; simpl in *.
+      2-3: destruct i; try constructor; lia. constructor. lia.
+    }
+    econstructor. constructor. {
+      constructor. simpl. constructor; auto.
+      cbn. do 2 constructor; auto. 2: do 2 constructor; lia.
+      all: intros; destruct i; simpl; constructor; auto; simpl in *.
+      2-3: destruct i; try constructor; lia. constructor. lia.
+    } auto.
+    {
+      constructor. simpl. rewrite (proj2 (scoped_ignores_sub 2) e); auto.
+    }
+    econstructor. constructor; auto. simpl. constructor.
+    {
+      constructor. simpl. rewrite (proj2 (scoped_ignores_sub 2) e); auto.
+    } auto.
+    econstructor. constructor; auto. simpl.
+    econstructor. constructor; auto. reflexivity. simpl.
+    econstructor. apply step_cons.
+    repeat rewrite renaming_is_subst.
+    repeat rewrite ren_up.
+    repeat rewrite subst_comp.
+    repeat rewrite up_comp.
+    repeat rewrite (proj2 (scoped_ignores_sub 2) e); auto.
+    apply frame_indep_nil with (Fs' := [FCons1
+     (EApp (EFun [x] e)
+        [a.[EFun [FVar; XVar]
+              (ECase (EVar 2) (PCons PVar PVar)
+                 (ECons (EApp (EVar 3) [EVar 0])
+                    (EApp (EFunId 2) [EVar 3; EVar 1])) ENil)/]])]) in H1. simpl in H1.
+    eapply transitive_eval.
+    rewrite (proj2 (scoped_ignores_sub 2) e) in H1; auto.
+    exact H1.
+   (** evaluate first element *)
+    econstructor. constructor. { auto. }
+    rewrite vclosed_ignores_sub; auto.
+    apply frame_indep_nil with (Fs' := [FCons2 (list_to_cons (map f l'))])
+       in DER. simpl in DER.
+    eapply transitive_eval. exact DER.
+    econstructor. constructor; auto. constructor.
+Qed.
+
+Theorem obj_foldr_on_meta_level :
+  forall l' l x y z e f
+  (VsCL : VALCLOSED l) (SCE : EXP 2 ⊢ e),
+  computes x e f -> cons_to_list l = Some l' ->
+  ⟨[], obj_foldr (EFun [y;z] (ECons (EApp (EFun [x] e) [EVar 1]) (EVar 2))) l ENil⟩
+ -->* list_to_cons (map f l').
+Proof.
+  induction l'; intros.
+  * assert (VALCLOSED (EFun [FVar; DVar; XVar]
+             (ECase (EVar 3) (PCons PVar PVar)
+                (EApp (EVar 3)
+                   [EVar 0; EApp (EFunId 2) [EVar 3; EVar 4; EVar 1]])
+                (EVar 2)))) as CLF1. {
+      do 2 constructor; auto. constructor; simpl; auto.
+      * do 2 constructor. lia.
+      * intros. destruct i. 2: destruct i. do 2 constructor. 1, 3: lia.
+        constructor; auto. simpl. intros.
+        do 2 constructor. lia.
+        simpl. intros. destruct i. 2: destruct i. 3: destruct i.
+        1-3: do 2 constructor. all: lia.
+      * simpl. do 2 constructor. lia.
+    }
+    assert (VALCLOSED (EFun [y; z] (ECons (EApp (EFun [x] e) [EVar 1]) (EVar 2)))). {
+      constructor. simpl. do 2 constructor.
+      * do 2 constructor. simpl. now apply (proj2 (scope_ext_app 5 2 ltac:(lia))).
+      * intros. simpl in H1. destruct i. do 2 constructor. all: lia.
+      * constructor. lia.
+    }
+    destruct l; simpl in H0; inversion H0.
+    2: { destruct (cons_to_list l2); inversion H0. }
+    unfold obj_map. cbn.
+    eexists. auto. eexists.
+    econstructor. constructor. cbn.
+    econstructor. constructor.
+    econstructor. constructor. auto.
+    repeat rewrite (proj2 (scoped_ignores_sub 2) e); auto.
+    econstructor. constructor; auto.
+    cbn.
+    econstructor. constructor; auto.
+    econstructor. constructor; auto.
+    {
+      constructor. auto.
+      constructor; auto.
+    } cbn.
+    econstructor. constructor; auto.
+    econstructor. apply red_case_false; auto.
+    constructor.
+  * destruct l; simpl in H0; inversion H0.
+    break_match_hyp; inversion H0. subst.
+    inversion VsCL. subst.
+    clear H0 H2 VsCL. specialize (IHl' _ _ y z _ _ H5 SCE H Heqo).
+    destruct IHl' as [VCL [k H']].
+    unfold obj_foldr in H'. inversion H'; subst.
+    1: { rewrite <- H3 in VCL. inversion_is_value. } clear H'.
+    inversion H0; subst. clear H0. simpl in H1.
+    (** eval first element (necessary before eexists): *)
+    specialize (H a) as [? [kk DER]].
+    (***)
+    unfold obj_map. split. { simpl. constructor; auto. }
+    assert (VALCLOSED (EFun [FVar; DVar; XVar]
+             (ECase (EVar 3) (PCons PVar PVar)
+                (EApp (EVar 3)
+                   [EVar 0; EApp (EFunId 2) [EVar 3; EVar 4; EVar 1]])
+                (EVar 2)))) as CLF1. {
+      do 2 constructor; auto. constructor; simpl; auto.
+      * do 2 constructor. lia.
+      * intros. destruct i. 2: destruct i. do 2 constructor. 1, 3: lia.
+        constructor; auto. simpl. intros.
+        do 2 constructor. lia.
+        simpl. intros. destruct i. 2: destruct i. 3: destruct i.
+        1-3: do 2 constructor. all: lia.
+      * simpl. do 2 constructor. lia.
+    }
+    assert (VALCLOSED (EFun [y; z] (ECons (EApp (EFun [x] e) [EVar 1]) (EVar 2)))) as CLVF2. {
+      constructor. simpl. do 2 constructor.
+      * do 2 constructor. simpl. now apply (proj2 (scope_ext_app 5 2 ltac:(lia))).
+      * intros. simpl in H1. destruct i. do 2 constructor. lia.
+        simpl in *. lia.
+      * constructor. lia.
+    }
+    eexists.
+    econstructor. constructor. cbn.
+    econstructor. constructor.
+    econstructor. constructor. auto.
+    repeat rewrite (proj2 (scoped_ignores_sub 2) e); auto.
+    rewrite (proj2 (scoped_ignores_sub 2) e) in H1; auto.
+    econstructor. constructor; auto. simpl.
+    econstructor. constructor; auto.
+    econstructor. constructor; auto.
+    {
+      constructor. auto.
+      constructor; auto.
+    } simpl.
+    econstructor. constructor; auto.
+    econstructor. constructor; auto. reflexivity. simpl.
+    repeat rewrite renaming_is_subst.
+    repeat rewrite ren_up.
+    repeat rewrite subst_comp.
+    repeat rewrite up_comp.
+    repeat rewrite (proj2 (scoped_ignores_sub 2) e); auto.
+    repeat rewrite vclosed_ignores_sub; auto.
+    rewrite vclosed_ignores_sub in H1; auto.
+    econstructor. constructor.
+    econstructor. constructor. auto.
+    econstructor. constructor; auto. simpl.
+    apply frame_indep_nil with (Fs' :=  [FApp2 (EFun [y; z] (ECons (EApp (EFun [x] e) [EVar 1]) (EVar 2))) [] [a]]) in H1. simpl in H1.
+    eapply transitive_eval. exact H1.
+   (** evaluate first element *)
+    econstructor. constructor; auto. simpl.
+    repeat rewrite (proj2 (scoped_ignores_sub 2) e); auto.
+    econstructor. constructor.
+    econstructor. constructor. { auto. }
+    apply frame_indep_nil with (Fs' := [FCons2 (list_to_cons (map f l'))])
+       in DER. simpl in DER.
+    eapply transitive_eval. exact DER.
+    econstructor. constructor; auto. constructor.
+Qed.
+
